Switch to the transitions library
Incorporates undefined behavior into Argosy's theorem statements. The
core framework compiles but not all of the soundness theorems are worked
out (and some of the statements might take into account undefined
behavior incorrectly). This version does add undefined behavior support
to Hoare logic, so that a specification includes undefined behavior when
the precondition is violated. This results in more complicated internal
proofs but is also more powerful.

src/Examples/StatDb/HoareProof.v
@@ -1,15 +1,24 @@
 Require Import Examples.StatDb.Impl.
 
-Require Import Helpers.RelationRewriting.
+From Transitions Require Import NonError.
 
 Require Import Spec.Hoare.
 Require Import Spec.HoareTactics.
 Require Import Spec.AbstractionSpec.
 
 Definition absr : relation DB.l.(State) Var.l.(State) unit :=
-  fun l s _ =>
-    fst s = fold_right plus 0 l /\
-    snd s = length l.
+  fun l res =>
+    match res with
+    | Val s _ =>
+      fst s = fold_right plus 0 l /\
+      snd s = length l
+    | Err _ _ => False
+    end.
+
+Instance absr_non_error : NonError absr.
+Proof.
+  compute; auto.
+Qed.
 
 Definition init_hspec : Specification InitStatus unit Var.State :=
   fun state =>
@@ -64,12 +73,18 @@ Definition recover_spec : Specification unit unit Var.State :=
 Lemma read_op_ok :
   forall i,
     proc_hspec Var.dynamics (read i) (op_spec Var.dynamics (Var.Read i)).
-Proof. intros. eapply op_spec_sound. Qed.
+Proof. intros. eapply op_spec_sound.
+       typeclasses eauto.
+       typeclasses eauto.
+Qed.
 
 Lemma write_op_ok :
   forall i v,
     proc_hspec Var.dynamics (write i v) (op_spec Var.dynamics (Var.Write i v)).
-Proof. intros. eapply op_spec_sound. Qed.
+Proof. intros. eapply op_spec_sound.
+       typeclasses eauto.
+       typeclasses eauto.
+Qed.
 
 Hint Resolve read_op_ok write_op_ok : core.
 
@@ -94,7 +109,12 @@ Ltac step :=
   unshelve (step_proc); simplify; finish.
 
 Lemma recover_cok : proc_hspec Var.dynamics (impl.(recover)) recover_spec.
-Proof. simpl. eapply ret_hspec; firstorder. Qed.
+Proof. simpl. eapply ret_hspec.
+       - typeclasses eauto.
+       - firstorder.
+         inversion H0; subst.
+         simpl; auto.
+Qed.
 
 Lemma recover_idempotent :
   idempotent (fun (t: unit) => recover_spec).
@@ -110,7 +130,10 @@ Proof. eapply proc_hspec_to_rspec; eauto. intros []; eauto. Qed.
 
 Lemma init_cok :
   proc_hspec Var.dynamics (impl.(init)) (init_hspec).
-Proof. eapply ret_hspec; firstorder. Qed.
+Proof. eapply ret_hspec.
+       - typeclasses eauto.
+       - firstorder.
+Qed.
 
 Lemma util_and3 (P Q R:Prop) :
   P -> Q -> R -> P /\ Q /\ R.
@@ -132,10 +155,10 @@ Ltac extract_pre H :=
   end.
 
 Lemma crash_step_simp s s' r :
-  Var.dynamics.(crash_step) s s' r ->
+  Var.dynamics.(crash_step) s (Val s' r) ->
   s' = (0, 0).
 Proof.
-  compute; auto.
+  compute; inversion 1; auto.
 Qed.
 
 Lemma op_step_crash T (op: Var.Op T) u s' r :
@@ -144,7 +167,7 @@ Lemma op_step_crash T (op: Var.Op T) u s' r :
 Proof.
   intros.
   hnf in H; propositional.
-  destruct H0; propositional.
+  destruct H0; propositional; eauto using crash_step_simp.
 Qed.
 
 Ltac extract_crash H :=
