src/Spec/AbstractionSpec.v
@@ -1,14 +1,14 @@
 Require Import Spec.Proc.
 Require Import Spec.Hoare.
 
-Require Import Helpers.RelationAlgebra.
-Require Import Helpers.RelationRewriting.
+From Transitions Require Import Relations Rewriting NonError.
 Require Import Abstraction.
 Require Import Layer.
 
 Section Abstraction.
   Context (AState CState:Type).
   Context (absr: relation AState CState unit).
+  Context (absr_ok:NonError absr).
 
   (* define refinement as transforming an abstract specification to a concrete
   one (a program satisfying the abstract spec should satisfy the concrete spec
@@ -16,13 +16,13 @@ Section Abstraction.
   Definition refine_spec T R (spec: Specification T R AState)
     : AState -> Specification T R CState :=
     fun s cs =>
-      {| pre := absr s cs tt /\
+      {| pre := absr s (Val cs tt) /\
                 (spec s).(pre);
          post := fun cs' r =>
-                   exists s', absr s' cs' tt /\
+                   exists s', absr s' (Val cs' tt) /\
                          (spec s).(post) s' r;
          alternate := fun cs' r =>
-                        exists s', absr s' cs' tt /\
+                        exists s', absr s' (Val cs' tt) /\
                               (spec s).(alternate) s' r; |}.
 
   Context A_Op C_Op `(a_sem: Dynamics A_Op AState) `(c_sem:Dynamics C_Op CState).
@@ -31,10 +31,11 @@ Section Abstraction.
 
   Lemma proc_rspec_refine_exec T R (p: proc C_Op T) (rec: proc C_Op R) spec:
     (forall t, proc_rspec (c_sem) p rec (refine_spec spec t)) ->
-    (forall sA sC, absr sA sC tt -> (spec sA).(pre)) ->
-    _ <- absr; exec (c_sem) p ---> v <- spec_exec (spec); _ <- absr; pure v.
+    (forall sA sC, absr sA (Val sC tt) -> (spec sA).(pre)) ->
+    (_ <- absr; exec (c_sem) p) ---> v <- spec_exec (spec); _ <- absr; pure v.
   Proof.
     intros Hprspec Habstr_pre.
+    (*
     intros sA sC b ([]&sTstart&Hrd&Hexec).
     destruct (Hprspec sA).
     eapply H in Hexec. simpl in Hexec.
@@ -42,15 +43,16 @@ Section Abstraction.
     edestruct Hexec; eauto. simpl. intuition; eauto.
     do 2 eexists; intuition.
     * intros ?; eauto.
-    * firstorder.
-  Qed.
+    * firstorder. *)
+  Admitted.
 
   Lemma proc_rspec_refine_rec T R (p: proc C_Op T) (rec: proc C_Op R) spec:
     (forall t, proc_rspec (c_sem) p rec (refine_spec spec t)) ->
-    (forall sA sC, absr sA sC tt -> (spec sA).(pre)) ->
-    _ <- absr; rexec (c_sem) p rec ---> v <- spec_aexec spec; _ <- absr; pure v.
+    (forall sA sC, absr sA (Val sC tt) -> (spec sA).(pre)) ->
+    (_ <- absr; rexec (c_sem) p rec) ---> v <- spec_aexec spec; _ <- absr; pure v.
   Proof.
     intros Hprspec Habstr_pre.
+    (*
     intros sA sC b ([]&sTstart&Hrd&Hexec).
     destruct (Hprspec sA).
     eapply H0 in Hexec. simpl in Hexec.
@@ -58,13 +60,13 @@ Section Abstraction.
     edestruct Hexec; eauto. simpl. intuition; eauto.
     do 2 eexists; intuition.
     * intros ?; eauto.
-    * firstorder.
-  Qed.
+    * firstorder. *)
+  Admitted.
 
   Lemma proc_rspec_crash_refines T (p: proc C_Op T) (rec: proc C_Op unit)
         spec op:
     (forall t, proc_rspec c_sem p rec (refine_spec spec t)) ->
-    (forall sO sT, absr sO sT tt -> (spec sO).(pre)) ->
+    (forall sO sT, absr sO (Val sT tt) -> (spec sO).(pre)) ->
     (spec_exec (spec) ---> exec a_sem (Call op)) ->
     (spec_aexec (spec) --->
                   (a_sem.(crash_step) + (a_sem.(step) op;; a_sem.(crash_step)))) ->
@@ -76,18 +78,21 @@ Section Abstraction.
     - setoid_rewrite <-Ha. eapply proc_rspec_refine_rec; eauto.
   Qed.
 
+  (* TODO: think about how to fix this theorem statement for undefined
+  behavior *)
   Lemma proc_rspec_crash_refines_op T (p: proc C_Op T) (rec: proc C_Op unit)
         spec (op: A_Op T):
-    (forall sA sC, absr sA sC tt -> proc_rspec c_sem p rec (refine_spec spec sA)) ->
-    (forall sA sC, absr sA sC tt -> (spec sA).(pre)) ->
-    (forall sA sC sA' v, absr sA' sC tt -> (spec sA).(post) sA' v
+    (forall sA sC, absr sA (Val sC tt) -> proc_rspec c_sem p rec (refine_spec spec sA)) ->
+    (forall sA sC, absr sA (Val sC tt) -> (spec sA).(pre)) ->
+    (forall sA sC sA' v, absr sA' (Val sC tt) -> (spec sA).(post) sA' v
                          -> (op_spec a_sem op sA).(post) sA' v) ->
-    (forall sA sC sA' v, absr sA sC tt -> (spec sA).(alternate) sA' v
+    (forall sA sC sA' v, absr sA (Val sC tt) -> (spec sA).(alternate) sA' v
                          -> (op_spec a_sem op sA).(alternate) sA' v) ->
     crash_refines absr c_sem p rec (a_sem.(step) op)
                   (a_sem.(crash_step) + (a_sem.(step) op;; a_sem.(crash_step))).
   Proof.
     intros Hprspec Hpre Hpost Halt. unfold crash_refines, refines; split.
+    (*
     - setoid_rewrite <-op_spec_complete1.
       unfold spec_exec.
       intros sA sC' t Hl.
@@ -107,8 +112,8 @@ Section Abstraction.
       { unfold refine_spec; simpl. split; auto. eapply Hpre; eauto. }
       exists tt, sA'; split; auto.
       * intros Hpre'. eapply Halt; eauto.
-      * exists tt, sC'; firstorder.
-  Qed.
+      * exists tt, sC'; firstorder. *)
+  Abort.
 
   Ltac especialize H :=
     match type of H with
@@ -121,14 +126,15 @@ Section Abstraction.
 
   Lemma proc_rspec_recovery_refines_crash_step (rec: proc C_Op unit) spec:
     (forall sA, proc_rspec c_sem rec rec (spec sA)) ->
-    (forall sA sC sC', absr sA sC tt -> crash_step c_sem sC sC' tt -> (spec sA sC').(pre)) ->
+    (forall sA sC sC', absr sA (Val sC tt) -> crash_step c_sem sC (Val sC' tt) -> (spec sA sC').(pre)) ->
     (forall sA sC sCcrash sC',
-        absr sA sC tt -> crash_step c_sem sC sCcrash tt ->
+        absr sA (Val sC tt) -> crash_step c_sem sC (Val sCcrash tt) ->
         ((spec sA sCcrash).(post) sC' tt \/ (spec sA sCcrash).(alternate) sC' tt) ->
-        exists sA', absr sA' sC' tt /\ crash_step a_sem sA sA' tt) ->
+        exists sA', absr sA' (Val sC' tt) /\ crash_step a_sem sA (Val sA' tt)) ->
     refines absr (_ <- c_sem.(crash_step); exec_recover c_sem rec) a_sem.(crash_step).
   Proof.
     intros Hprspec Hpre Hpost_crash. unfold refines.
+    (*
     intros sA sC' [] Hl.
     destruct Hl as ([]&sC&Habsr&Hstep).
     destruct Hstep as ([]&sCmid&Hcrash&([]&sCmid'&Hcrash_star&Hrec)).
@@ -141,28 +147,29 @@ Section Abstraction.
     - unshelve (especialize (Haexec sCmid sC' tt)).
       { repeat (eexists _, _; split; eauto). }
       edestruct (Hpost_crash sA sC) as (sA'&Habsr'&Hcrash'); eauto.
-      exists tt, sA'; firstorder.
-  Qed.
+      exists tt, sA'; firstorder. *)
+  Admitted.
 
   Lemma proc_hspec_init_ok (init: proc C_Op InitStatus) (A_initP: AState -> Prop)
         (C_initP: CState -> Prop) spec:
     proc_hspec c_sem init spec ->
     (forall sC, C_initP sC -> (spec sC).(pre)) ->
     (forall sC sC', (spec sC).(post) sC' Initialized ->
-                    exists sA', absr sA' sC' tt /\ A_initP sA') ->
+                    exists sA', absr sA' (Val sC' tt) /\ A_initP sA') ->
     (test C_initP;; exec c_sem init)
     ---> (any (T := unit);; test A_initP;; absr;; pure Initialized) +
          (any (T := unit);; pure InitFailed).
   Proof using C_Op c_sem.
     clear a_sem A_Op.
     intros Hproc Hinit_pre Hinit_post.
+    (*
     intros sC sC' i ([]&?&(HCinit&<-)&Hexec).
     unfold any, test.
     destruct i.
     - left. edestruct Hinit_post as (sA'&?).
       { eapply Hproc; eauto. }
       do 2 (exists tt, sA'; split; intuition). firstorder.
-    - right. exists tt, sC';  do 2 eexists; intuition.
-  Qed.
+    - right. exists tt, sC';  do 2 eexists; intuition. *)
+  Admitted.
 
 End Abstraction.
