src/Lib.v
@@ -2,8 +2,8 @@ From Coq Require Export List.
 From Coq Require Export Omega.
 
 From Classes Require Export Classes.
-Require Export Helpers.RelationAlgebra.
-Require Export Tactical.ProofAutomation.
+From Transitions Require Export Relations.
+From Tactical Require Export ProofAutomation.
 
 Require Export Spec.Proc.
 Require Export Spec.ProcTheorems.
